formal/lean/Hegemon/Release/CiReleaseGate.lean
@@ -5,17 +5,29 @@ namespace CiReleaseGate
 inductive CiReleaseGateReject where
   | dependencyAuditMissing
   | formalCoreMissing
+  | securityAdversarialMissing
+  | nativeBackendSecurityMissing
   | releaseBuildMissing
   | releaseBuildDependencyMissing
+  | releaseBuildSecurityAdversarialDependencyMissing
+  | releaseBuildNativeBackendSecurityDependencyMissing
   | releaseBinaryAuditMissing
+  | tagReleaseNativeBackendReviewMissing
+  | tagReleaseNativeBackendPostureMissing
 deriving DecidableEq, Repr
 
 structure CiReleaseGateInput where
   dependencyAuditJob : Bool
   formalCoreJob : Bool
+  securityAdversarialJob : Bool
+  nativeBackendSecurityJob : Bool
   releaseBuildJob : Bool
   releaseBuildNeedsSecurityGates : Bool
+  releaseBuildNeedsSecurityAdversarial : Bool
+  releaseBuildNeedsNativeBackendSecurity : Bool
   releaseBinaryAuditStep : Bool
+  tagReleaseNativeBackendReviewStep : Bool
+  tagReleaseNativeBackendPostureStep : Bool
 deriving DecidableEq, Repr
 
 def evaluateCiReleaseGate
@@ -24,12 +36,26 @@ def evaluateCiReleaseGate
     Except.error CiReleaseGateReject.dependencyAuditMissing
   else if input.formalCoreJob = false then
     Except.error CiReleaseGateReject.formalCoreMissing
+  else if input.securityAdversarialJob = false then
+    Except.error CiReleaseGateReject.securityAdversarialMissing
+  else if input.nativeBackendSecurityJob = false then
+    Except.error CiReleaseGateReject.nativeBackendSecurityMissing
   else if input.releaseBuildJob = false then
     Except.error CiReleaseGateReject.releaseBuildMissing
   else if input.releaseBuildNeedsSecurityGates = false then
     Except.error CiReleaseGateReject.releaseBuildDependencyMissing
+  else if input.releaseBuildNeedsSecurityAdversarial = false then
+    Except.error
+      CiReleaseGateReject.releaseBuildSecurityAdversarialDependencyMissing
+  else if input.releaseBuildNeedsNativeBackendSecurity = false then
+    Except.error
+      CiReleaseGateReject.releaseBuildNativeBackendSecurityDependencyMissing
   else if input.releaseBinaryAuditStep = false then
     Except.error CiReleaseGateReject.releaseBinaryAuditMissing
+  else if input.tagReleaseNativeBackendReviewStep = false then
+    Except.error CiReleaseGateReject.tagReleaseNativeBackendReviewMissing
+  else if input.tagReleaseNativeBackendPostureStep = false then
+    Except.error CiReleaseGateReject.tagReleaseNativeBackendPostureMissing
   else
     Except.ok ()
 
@@ -47,32 +73,53 @@ def ciReleaseGateRejection
 def ciReleaseGatePreconditions (input : CiReleaseGateInput) : Bool :=
   input.dependencyAuditJob &&
     input.formalCoreJob &&
+    input.securityAdversarialJob &&
+    input.nativeBackendSecurityJob &&
     input.releaseBuildJob &&
     input.releaseBuildNeedsSecurityGates &&
-    input.releaseBinaryAuditStep
+    input.releaseBuildNeedsSecurityAdversarial &&
+    input.releaseBuildNeedsNativeBackendSecurity &&
+    input.releaseBinaryAuditStep &&
+    input.tagReleaseNativeBackendReviewStep &&
+    input.tagReleaseNativeBackendPostureStep
 
 theorem accepts_iff_ci_release_gate_preconditions
     (input : CiReleaseGateInput) :
     ciReleaseGateAccepts input = ciReleaseGatePreconditions input := by
   cases input with
-  | mk dependencyAuditJob formalCoreJob releaseBuildJob
-      releaseBuildNeedsSecurityGates releaseBinaryAuditStep =>
+  | mk dependencyAuditJob formalCoreJob securityAdversarialJob
+      nativeBackendSecurityJob releaseBuildJob releaseBuildNeedsSecurityGates
+      releaseBuildNeedsSecurityAdversarial
+      releaseBuildNeedsNativeBackendSecurity releaseBinaryAuditStep
+      tagReleaseNativeBackendReviewStep tagReleaseNativeBackendPostureStep =>
       unfold ciReleaseGateAccepts ciReleaseGatePreconditions
         evaluateCiReleaseGate
       cases dependencyAuditJob <;>
         cases formalCoreJob <;>
+        cases securityAdversarialJob <;>
+        cases nativeBackendSecurityJob <;>
         cases releaseBuildJob <;>
         cases releaseBuildNeedsSecurityGates <;>
+        cases releaseBuildNeedsSecurityAdversarial <;>
+        cases releaseBuildNeedsNativeBackendSecurity <;>
         cases releaseBinaryAuditStep <;>
+        cases tagReleaseNativeBackendReviewStep <;>
+        cases tagReleaseNativeBackendPostureStep <;>
         rfl
 
 def completeCiReleaseGate : CiReleaseGateInput :=
   {
     dependencyAuditJob := true,
     formalCoreJob := true,
+    securityAdversarialJob := true,
+    nativeBackendSecurityJob := true,
     releaseBuildJob := true,
     releaseBuildNeedsSecurityGates := true,
-    releaseBinaryAuditStep := true
+    releaseBuildNeedsSecurityAdversarial := true,
+    releaseBuildNeedsNativeBackendSecurity := true,
+    releaseBinaryAuditStep := true,
+    tagReleaseNativeBackendReviewStep := true,
+    tagReleaseNativeBackendPostureStep := true
   }
 
 def missingDependencyAuditJob : CiReleaseGateInput :=
@@ -81,14 +128,32 @@ def missingDependencyAuditJob : CiReleaseGateInput :=
 def missingFormalCoreJob : CiReleaseGateInput :=
   { completeCiReleaseGate with formalCoreJob := false }
 
+def missingSecurityAdversarialJob : CiReleaseGateInput :=
+  { completeCiReleaseGate with securityAdversarialJob := false }
+
+def missingNativeBackendSecurityJob : CiReleaseGateInput :=
+  { completeCiReleaseGate with nativeBackendSecurityJob := false }
+
 def missingReleaseBuildJob : CiReleaseGateInput :=
   { completeCiReleaseGate with releaseBuildJob := false }
 
 def missingReleaseBuildDependency : CiReleaseGateInput :=
   { completeCiReleaseGate with releaseBuildNeedsSecurityGates := false }
 
+def missingReleaseBuildSecurityAdversarialDependency : CiReleaseGateInput :=
+  { completeCiReleaseGate with releaseBuildNeedsSecurityAdversarial := false }
+
+def missingReleaseBuildNativeBackendSecurityDependency : CiReleaseGateInput :=
+  { completeCiReleaseGate with releaseBuildNeedsNativeBackendSecurity := false }
+
 def missingReleaseBinaryAuditStep : CiReleaseGateInput :=
   { completeCiReleaseGate with releaseBinaryAuditStep := false }
+
+def missingTagReleaseNativeBackendReviewStep : CiReleaseGateInput :=
+  { completeCiReleaseGate with tagReleaseNativeBackendReviewStep := false }
+
+def missingTagReleaseNativeBackendPostureStep : CiReleaseGateInput :=
+  { completeCiReleaseGate with tagReleaseNativeBackendPostureStep := false }
 
 theorem complete_ci_release_gate_accepts :
     evaluateCiReleaseGate completeCiReleaseGate = Except.ok () := by
@@ -115,42 +180,217 @@ theorem release_build_missing_rejects_after_security_jobs
     {input : CiReleaseGateInput}
     (dependency : input.dependencyAuditJob = true)
     (formalCore : input.formalCoreJob = true)
+    (securityAdversarial : input.securityAdversarialJob = true)
+    (nativeBackendSecurity : input.nativeBackendSecurityJob = true)
     (releaseBuild : input.releaseBuildJob = false) :
     evaluateCiReleaseGate input =
       Except.error CiReleaseGateReject.releaseBuildMissing := by
   unfold evaluateCiReleaseGate
-  simp [dependency, formalCore, releaseBuild]
+  simp [
+    dependency,
+    formalCore,
+    securityAdversarial,
+    nativeBackendSecurity,
+    releaseBuild
+  ]
 
 theorem release_build_dependency_missing_rejects_after_jobs
     {input : CiReleaseGateInput}
     (dependency : input.dependencyAuditJob = true)
     (formalCore : input.formalCoreJob = true)
+    (securityAdversarial : input.securityAdversarialJob = true)
+    (nativeBackendSecurity : input.nativeBackendSecurityJob = true)
     (releaseBuild : input.releaseBuildJob = true)
     (needsSecurity : input.releaseBuildNeedsSecurityGates = false) :
     evaluateCiReleaseGate input =
       Except.error CiReleaseGateReject.releaseBuildDependencyMissing := by
   unfold evaluateCiReleaseGate
-  simp [dependency, formalCore, releaseBuild, needsSecurity]
+  simp [
+    dependency,
+    formalCore,
+    securityAdversarial,
+    nativeBackendSecurity,
+    releaseBuild,
+    needsSecurity
+  ]
 
 theorem release_binary_audit_missing_rejects_after_security_jobs
     {input : CiReleaseGateInput}
     (dependency : input.dependencyAuditJob = true)
     (formalCore : input.formalCoreJob = true)
+    (securityAdversarial : input.securityAdversarialJob = true)
+    (nativeBackendSecurity : input.nativeBackendSecurityJob = true)
     (releaseBuild : input.releaseBuildJob = true)
     (needsSecurity : input.releaseBuildNeedsSecurityGates = true)
+    (needsAdversarial :
+      input.releaseBuildNeedsSecurityAdversarial = true)
+    (needsNativeBackend :
+      input.releaseBuildNeedsNativeBackendSecurity = true)
     (binaryAudit : input.releaseBinaryAuditStep = false) :
     evaluateCiReleaseGate input =
       Except.error CiReleaseGateReject.releaseBinaryAuditMissing := by
   unfold evaluateCiReleaseGate
-  simp [dependency, formalCore, releaseBuild, needsSecurity, binaryAudit]
+  simp [
+    dependency,
+    formalCore,
+    securityAdversarial,
+    nativeBackendSecurity,
+    releaseBuild,
+    needsSecurity,
+    needsAdversarial,
+    needsNativeBackend,
+    binaryAudit
+  ]
+
+theorem security_adversarial_missing_rejects_after_formal_core
+    {input : CiReleaseGateInput}
+    (dependency : input.dependencyAuditJob = true)
+    (formalCore : input.formalCoreJob = true)
+    (securityAdversarial : input.securityAdversarialJob = false) :
+    evaluateCiReleaseGate input =
+      Except.error CiReleaseGateReject.securityAdversarialMissing := by
+  unfold evaluateCiReleaseGate
+  simp [dependency, formalCore, securityAdversarial]
+
+theorem native_backend_security_missing_rejects_after_adversarial
+    {input : CiReleaseGateInput}
+    (dependency : input.dependencyAuditJob = true)
+    (formalCore : input.formalCoreJob = true)
+    (securityAdversarial : input.securityAdversarialJob = true)
+    (nativeBackendSecurity : input.nativeBackendSecurityJob = false) :
+    evaluateCiReleaseGate input =
+      Except.error CiReleaseGateReject.nativeBackendSecurityMissing := by
+  unfold evaluateCiReleaseGate
+  simp [dependency, formalCore, securityAdversarial, nativeBackendSecurity]
+
+theorem release_build_security_adversarial_dependency_missing_rejects
+    {input : CiReleaseGateInput}
+    (dependency : input.dependencyAuditJob = true)
+    (formalCore : input.formalCoreJob = true)
+    (securityAdversarial : input.securityAdversarialJob = true)
+    (nativeBackendSecurity : input.nativeBackendSecurityJob = true)
+    (releaseBuild : input.releaseBuildJob = true)
+    (needsSecurity : input.releaseBuildNeedsSecurityGates = true)
+    (needsAdversarial :
+      input.releaseBuildNeedsSecurityAdversarial = false) :
+    evaluateCiReleaseGate input =
+      Except.error
+        CiReleaseGateReject.releaseBuildSecurityAdversarialDependencyMissing := by
+  unfold evaluateCiReleaseGate
+  simp [
+    dependency,
+    formalCore,
+    securityAdversarial,
+    nativeBackendSecurity,
+    releaseBuild,
+    needsSecurity,
+    needsAdversarial
+  ]
+
+theorem release_build_native_backend_security_dependency_missing_rejects
+    {input : CiReleaseGateInput}
+    (dependency : input.dependencyAuditJob = true)
+    (formalCore : input.formalCoreJob = true)
+    (securityAdversarial : input.securityAdversarialJob = true)
+    (nativeBackendSecurity : input.nativeBackendSecurityJob = true)
+    (releaseBuild : input.releaseBuildJob = true)
+    (needsSecurity : input.releaseBuildNeedsSecurityGates = true)
+    (needsAdversarial :
+      input.releaseBuildNeedsSecurityAdversarial = true)
+    (needsNativeBackend :
+      input.releaseBuildNeedsNativeBackendSecurity = false) :
+    evaluateCiReleaseGate input =
+      Except.error
+        CiReleaseGateReject.releaseBuildNativeBackendSecurityDependencyMissing := by
+  unfold evaluateCiReleaseGate
+  simp [
+    dependency,
+    formalCore,
+    securityAdversarial,
+    nativeBackendSecurity,
+    releaseBuild,
+    needsSecurity,
+    needsAdversarial,
+    needsNativeBackend
+  ]
+
+theorem tag_release_native_backend_review_missing_rejects
+    {input : CiReleaseGateInput}
+    (dependency : input.dependencyAuditJob = true)
+    (formalCore : input.formalCoreJob = true)
+    (securityAdversarial : input.securityAdversarialJob = true)
+    (nativeBackendSecurity : input.nativeBackendSecurityJob = true)
+    (releaseBuild : input.releaseBuildJob = true)
+    (needsSecurity : input.releaseBuildNeedsSecurityGates = true)
+    (needsAdversarial :
+      input.releaseBuildNeedsSecurityAdversarial = true)
+    (needsNativeBackend :
+      input.releaseBuildNeedsNativeBackendSecurity = true)
+    (binaryAudit : input.releaseBinaryAuditStep = true)
+    (review : input.tagReleaseNativeBackendReviewStep = false) :
+    evaluateCiReleaseGate input =
+      Except.error
+        CiReleaseGateReject.tagReleaseNativeBackendReviewMissing := by
+  unfold evaluateCiReleaseGate
+  simp [
+    dependency,
+    formalCore,
+    securityAdversarial,
+    nativeBackendSecurity,
+    releaseBuild,
+    needsSecurity,
+    needsAdversarial,
+    needsNativeBackend,
+    binaryAudit,
+    review
+  ]
+
+theorem tag_release_native_backend_posture_missing_rejects
+    {input : CiReleaseGateInput}
+    (dependency : input.dependencyAuditJob = true)
+    (formalCore : input.formalCoreJob = true)
+    (securityAdversarial : input.securityAdversarialJob = true)
+    (nativeBackendSecurity : input.nativeBackendSecurityJob = true)
+    (releaseBuild : input.releaseBuildJob = true)
+    (needsSecurity : input.releaseBuildNeedsSecurityGates = true)
+    (needsAdversarial :
+      input.releaseBuildNeedsSecurityAdversarial = true)
+    (needsNativeBackend :
+      input.releaseBuildNeedsNativeBackendSecurity = true)
+    (binaryAudit : input.releaseBinaryAuditStep = true)
+    (review : input.tagReleaseNativeBackendReviewStep = true)
+    (posture : input.tagReleaseNativeBackendPostureStep = false) :
+    evaluateCiReleaseGate input =
+      Except.error
+        CiReleaseGateReject.tagReleaseNativeBackendPostureMissing := by
+  unfold evaluateCiReleaseGate
+  simp [
+    dependency,
+    formalCore,
+    securityAdversarial,
+    nativeBackendSecurity,
+    releaseBuild,
+    needsSecurity,
+    needsAdversarial,
+    needsNativeBackend,
+    binaryAudit,
+    review,
+    posture
+  ]
 
 theorem dependency_audit_precedes_all_missing :
     evaluateCiReleaseGate {
       dependencyAuditJob := false,
       formalCoreJob := false,
+      securityAdversarialJob := false,
+      nativeBackendSecurityJob := false,
       releaseBuildJob := false,
       releaseBuildNeedsSecurityGates := false,
-      releaseBinaryAuditStep := false
+      releaseBuildNeedsSecurityAdversarial := false,
+      releaseBuildNeedsNativeBackendSecurity := false,
+      releaseBinaryAuditStep := false,
+      tagReleaseNativeBackendReviewStep := false,
+      tagReleaseNativeBackendPostureStep := false
     } = Except.error CiReleaseGateReject.dependencyAuditMissing := by
   rfl
 
